compiler/backend/proofs/clos_to_bvlProofScript.sml
@@ -1429,7 +1429,7 @@ Proof
      \\ res_tac \\ fs [] \\ rveq \\ fs []
      \\ rw [] \\ res_tac \\ fs []
      \\ imp_res_tac LIST_REL_LENGTH \\ fs [])
-  \\ Cases_on `?i. op = EqualInt i` THEN1
+  \\ Cases_on `?i. op = EqualConst i` THEN1
     (srw_tac[][closSemTheory.do_app_def] \\ fs [] \\ every_case_tac \\ fs [])
   \\ Cases_on `op = Install` THEN1 fs[closSemTheory.do_app_def]
   \\ Cases_on `op = Equal` THEN1
@@ -1645,7 +1645,7 @@ val do_app_err = Q.prove(
    ⇒
    ∃e. do_app (compile_op op) ys t1 = Rerr e ∧
        exc_rel (v_rel s1.max_app f t1.refs t1.code) err e`,
-  Cases_on `?i. op = EqualInt i` THEN1
+  Cases_on `?i. op = EqualConst i` THEN1
     (srw_tac[][closSemTheory.do_app_def] \\ fs [] \\ every_case_tac \\ fs []) >>
   Cases_on `?tag. op = ConsExtend tag`
   >- (
